Seal definitions of proph_ag

nola/iris/proph_ag.v
@@ -24,16 +24,33 @@ Section proph_ag.
   Context `{!proph_agG TY Σ, !prophGS TY Σ}.
 
   (** Value observer *)
-  Definition val_obs γ X x : iProp Σ := ghost_var γ (1/2) (Anyty X x).
+  Local Definition val_obs_def γ X x : iProp Σ := ghost_var γ (1/2) (Anyty X x).
+  Local Lemma val_obs_aux : seal val_obs_def. Proof. by eexists. Qed.
+  Definition val_obs := val_obs_aux.(unseal).
+  Local Lemma val_obs_unseal : val_obs = val_obs_def.
+  Proof. exact: seal_eq. Qed.
+
   (** Double value observer *)
-  Definition val_obs2 γ X x : iProp Σ := ghost_var γ 1 (Anyty X x).
+  Local Definition val_obs2 γ X x : iProp Σ := ghost_var γ 1 (Anyty X x).
+
   (** Prophecy controller *)
-  Definition proph_ctrl γ X x (ξ : prvar X) : iProp Σ :=
-    (val_obs γ X x ∗ 1:[ξ]) ∨
+  Local Definition proph_ctrl_def γ X x (ξ : prvar X) : iProp Σ :=
+    (val_obs_def γ X x ∗ 1:[ξ]) ∨
     ((∃ x', val_obs2 γ X x') ∗ ⟨π, π ξ = x⟩).
+  Local Lemma proph_ctrl_aux : seal proph_ctrl_def. Proof. by eexists. Qed.
+  Definition proph_ctrl := proph_ctrl_aux.(unseal).
+  Local Lemma proph_ctrl_unseal : proph_ctrl = proph_ctrl_def.
+  Proof. exact: seal_eq. Qed.
+
+  (** [val_obs] and [proph_ctrl] are timeless *)
+  #[export] Instance val_obs_timeless {γ X x} : Timeless (val_obs γ X x).
+  Proof. rewrite val_obs_unseal. exact _. Qed.
+  #[export] Instance proph_ctrl_timeless {γ X x ξ} :
+    Timeless (proph_ctrl γ X x ξ).
+  Proof. rewrite proph_ctrl_unseal. exact _. Qed.
 
   (** [val_obs] and [val_obs2] can't coexist *)
-  Lemma vo_vo2 {γ X x x'} : val_obs γ X x -∗ val_obs2 γ X x' -∗ False.
+  Local Lemma vo_vo2 {γ X x x'} : val_obs_def γ X x -∗ val_obs2 γ X x' -∗ False.
   Proof.
     iIntros "vo vo'". by iDestruct (ghost_var_valid_2 with "vo vo'") as %[? _].
   Qed.
@@ -42,14 +59,16 @@ Section proph_ag.
   Lemma vo_pc_alloc {X x} {ξ : prvar X} :
     1:[ξ] ==∗ ∃ γ, val_obs γ X x ∗ proph_ctrl γ X x ξ.
   Proof.
-    iIntros "ξ". iMod ghost_var_alloc as (γ) "[vo vo']". iModIntro. iExists _.
-    iFrame "vo". iLeft. iFrame.
+    rewrite val_obs_unseal proph_ctrl_unseal. iIntros "ξ".
+    iMod ghost_var_alloc as (γ) "[vo vo']". iModIntro. iExists _. iFrame "vo".
+    iLeft. iFrame.
   Qed.
 
   (** Agreement between [val_obs] and [proph_ctrl] *)
   Lemma vo_pc_agree {γ X x x' ξ} :
     val_obs γ X x -∗ proph_ctrl γ X x' ξ -∗ ⌜x = x'⌝.
   Proof.
+    rewrite val_obs_unseal proph_ctrl_unseal.
     iIntros "vo [[vo' _]|[[% vo2] _]]"; last first.
     { iDestruct (vo_vo2 with "vo vo2") as %[]. }
     iDestruct (ghost_var_agree with "vo vo'") as %?. by simplify_eq.
@@ -59,6 +78,7 @@ Section proph_ag.
   Lemma vo_pc_update {γ X x x' y ξ} :
     val_obs γ X x -∗ proph_ctrl γ X x' ξ ==∗ val_obs γ X y ∗ proph_ctrl γ X y ξ.
   Proof.
+    rewrite val_obs_unseal proph_ctrl_unseal.
     iIntros "vo [[vo' ξ]|[[% vo2] _]]"; last first.
     { iDestruct (vo_vo2 with "vo vo2") as %[]. }
     iMod (ghost_var_update_2 with "vo vo'") as "[$ vo]"; [by rewrite Qp.div_2|].
@@ -71,6 +91,7 @@ Section proph_ag.
     q:∗[ηl] -∗ val_obs γ X x -∗ proph_ctrl γ X x' ξ =[proph_wsat]=∗
       q:∗[ηl] ∗ ⟨π, π ξ = aπ π⟩ ∗ (∀ y, ⟨π, aπ π = y⟩ -∗ proph_ctrl γ X y ξ).
   Proof.
+    rewrite val_obs_unseal proph_ctrl_unseal.
     iIntros "% ηl vo [[vo' ξ]|[[% vo2] _]]"; last first.
     { iDestruct (vo_vo2 with "vo vo2") as %[]. }
     iMod (proph_resolve_dep with "ξ ηl") as "[$ #obs]"; [done|]. iModIntro.
@@ -81,5 +102,8 @@ Section proph_ag.
   (** Resolve the prophecy of [proph_ctrl] *)
   Lemma pc_resolve {γ X x} ξ :
     proph_ctrl γ X x ξ =[proph_wsat]=∗ ⟨π, π ξ = x⟩.
-  Proof. iIntros "[[_ ξ]|[_ $]]"; [|done]. iApply (proph_resolve with "ξ"). Qed.
+  Proof.
+    rewrite proph_ctrl_unseal. iIntros "[[_ ξ]|[_ $]]"; [|done].
+    iApply (proph_resolve with "ξ").
+  Qed.
 End proph_ag.
